\section{Linear algebra}

\begin{definition}[Rings]

\end{definition}

\begin{definition}[Fields]

\end{definition}

\begin{theorem}[Sherman-Morrison-Woodbury formula]
    Let \(M\) be a \(n \times n\) matrix, \(U\) and \(V\) be \(n \times k\) matrices.
    Suppose that \(M\) is non-singular. 
    Then
    \begin{enumerate}[label = (\arabic*)]
        \item \(M + UV^T\) is non-singular iff \(I + V^TM^{-1}U\) is non-singular;
        \item If \(M + UV^T\) is non-singular, then
        \[
            (M + UV^T)^{-1} = M^{-1} - M^{-1}U(I + V^TM^{-1}U)^{-1}V^TM^{-1}.
        \]
    \end{enumerate}
\end{theorem}

\begin{proof}
    For (1).

    For (2), it suffices to verify that 
    \[
        (M + UV^T)(M^{-1} - M^{-1}U(I + V^TM^{-1}U)^{-1}V^TM^{-1}) = I.
    \]
    Let \(A \coloneqq (I + V^TM^{-1}U)\), then
    \begin{align*}
        &(M + UV^T)(M^{-1} - M^{-1}U(I + V^TM^{-1}U)^{-1}V^TM^{-1})\\
        = \, &(M + UV^T)(M^{-1} - M^{-1}UA^{-1}V^TM^{-1})\\
        = \, &(MM^{-1} - MM^{-1}UA^{-1}V^TM^{-1}) + UV^T(M^{-1} - M^{-1}UA^{-1}V^TM^{-1}) \\
        = \, &(I - UA^{-1}V^TM^{-1}) + UV^T(M^{-1} - M^{-1}UA^{-1}V^TM^{-1}) \\
        = \, &(I - UA^{-1}V^TM^{-1}) + (UV^TM^{-1} - UV^TM^{-1}UA^{-1}V^TM^{-1}) \\
        = \, &(I + UV^TM^{-1}) - (UA^{-1}V^TM^{-1} + UV^TM^{-1}UA^{-1}V^TM^{-1}) \\
        = \, &(I + UV^TM^{-1}) - U(A^{-1}V^TM^{-1} + V^TM^{-1}UA^{-1}V^TM^{-1}) \\
        = \, &(I + UV^TM^{-1}) - U(I + V^TM^{-1}U)(A^{-1}V^TM^{-1}) \\
        = \, &(I + UV^TM^{-1}) - UAA^{-1}V^TM^{-1} \\
        = \, &(I + UV^TM^{-1}) - UIV^TM^{-1} =  I + UV^TM^{-1} - UV^TM^{-1} = I. \qedhere \\
    \end{align*}
\end{proof}

\begin{corollary}
    \label{cor:1}
    Let \(M\) be a non-singular matrix and let \(N\) be its inverse, 
    \(M'\) be a matrix which is identical to \(M\) except that \(M'_{S, S} \neq M_{S, S}\)
    and \(\Delta \coloneqq M'_{S, S} - M_{S, S}\).
    If \(M'\) is non-singular, then
    \[
        M'^{-1} = N - N_{*, S}(I + \Delta N_{S, S})^{-1}\Delta N_{S, *}.
    \]
\end{corollary}